experiments added

experiments/fqueue/Quark_Fqueue.ml
@@ -1,112 +1,99 @@
-module Queue: sig
-  type t
-  type op = Enqueue of int | Dequeue
-  val empty : t
-  val peek : t -> int option
-  val app_op: (int * op) -> t -> t
-  val merge : t -> t -> t -> t
-end = struct
 
-  type t = (int * int) list * (int * int) list
-  type op = Enqueue of int | Dequeue
+type s = | S of ((Z.t * Z.t) list) * ((Z.t * Z.t) list)
 
-  let empty = ([], [])
-  let norm q = match q with
-    | [], l -> (List.rev l, [])
-    | _ -> q
-  let to_list (front, back) = front @ (List.rev back)
+let empty = S ([], [])
+let (norm: s -> s) = fun q -> match q with
+  | S ([], l) -> S (List.rev l, [])
+  | _ -> q
 
-  let enqueue (front, back) a = (front, a::back)
+let (to_list: s -> (Z.t * Z.t) list) = fun (S (front, back)) -> front @ (List.rev back)
 
-  let dequeue q = match q with
-    | [], [] -> (None, ([], []))
-    | [], x::xs -> let (l1, l2) = norm q in
-      (Some (List.hd l1), ((List.tl l1), l2))
-    | x::xs, l -> (Some x, (xs, l))
+let (enqueue: (Z.t * Z.t) -> s -> s) = fun a st -> match st with
+  | S (front, back) -> S (front, a::back)
 
-  let app_op op st = match op with
-    | (id, Enqueue x) -> enqueue st (id, x)
-    | (_, Dequeue) -> snd (dequeue st)
+let (dequeue: s -> (((Z.t * Z.t) option) * s)) = fun q -> match q with
+  | S ([], []) -> (None, S ([], []))
+  | S ([], x::xs) -> let (S (l1, l2)) = norm q in
+    (Some (List.hd l1), S ((List.tl l1), l2))
+  | S (x::xs, l) -> (Some x, S (xs, l))
 
-  let peek q = match q with
-    | [], [] -> None
-    | [], x::xs -> Some (fst (List.hd (fst (norm q))))
-    | x::xs, _ -> Some (fst x)
+let peek q = match q with
+  | S ([], []) -> None
+  | S ([], x::xs) -> let (S (l1, l2)) = norm q in Some (fst (List.hd l1))
+  | S (x::xs, _) -> Some (fst x)
 
-  module PairSet = Set.Make(struct
-      type t = (int * int)
-      let compare a b = if a = b then 0 else (if a < b then 1 else -1) end)
+module PairSet = Set.Make(struct
+    type t = (Z.t * Z.t)
+    let compare a b = if a = b then 0 else (if a < b then 1 else -1) end)
 
-  module PairPairSet = Set.Make(struct
-      type t = ((int * int) * (int * int))
-      let compare a b = if a = b then 0 else (if a < b then 1 else -1) end)
+module PairPairSet = Set.Make(struct
+    type t = ((Z.t * Z.t) * (Z.t * Z.t))
+    let compare a b = if a = b then 0 else (if a < b then 1 else -1) end)
 
-  let r_mem q =
-    let q_list = to_list q in
-    List.fold_left (fun acc x -> PairSet.union (PairSet.singleton x) acc) PairSet.empty q_list
+let r_mem q =
+  let q_list = to_list q in
+  List.fold_left (fun acc x -> PairSet.union (PairSet.singleton x) acc) PairSet.empty q_list
 
-  let r_cross x xs =
-    let acc_list = PairSet.elements xs in
-    List.fold_left (fun acc a -> PairPairSet.union acc (PairPairSet.singleton (x, a))) PairPairSet.empty acc_list
+let r_cross x xs =
+  let acc_list = PairSet.elements xs in
+  List.fold_left (fun acc a -> PairPairSet.union acc (PairPairSet.singleton (x, a))) PairPairSet.empty acc_list
 
-  let rec r_cross_sets s1 s2 =
-    let s1_list = PairSet.elements s1 in
-    List.fold_left (fun acc x -> PairPairSet.union acc (r_cross x s2)) PairPairSet.empty s1_list
+let rec r_cross_sets s1 s2 =
+  let s1_list = PairSet.elements s1 in
+  List.fold_left (fun acc x -> PairPairSet.union acc (r_cross x s2)) PairPairSet.empty s1_list
 
-  let rec r_ob q = match (to_list q) with
-    | [] -> PairPairSet.empty
-    | x::xs -> PairPairSet.union (r_cross x (r_mem (xs, []))) (r_ob (xs, []))
+let rec r_ob q = match (to_list q) with
+  | [] -> PairPairSet.empty
+  | x::xs -> PairPairSet.union (r_cross x (r_mem (S (xs, [])))) (r_ob (S (xs, [])))
 
-  let abstract q = (r_mem q, r_ob q)
+let abstract q = (r_mem q, r_ob q)
 
-  let merge_rels lca a b diff inter union =
-    let ixn = (inter (inter a b) lca) in
-    let diff_a = diff a lca in
-    let diff_b = diff b lca in
-    union (union diff_a diff_b) ixn
+let merge_rels lca a b diff inter union =
+  let ixn = (inter (inter a b) lca) in
+  let diff_a = diff a lca in
+  let diff_b = diff b lca in
+  union (union diff_a diff_b) ixn
 
-  let merge_r lca a b =
-    let (lca_mem, lca_ob) = abstract lca in
-    let (a_mem, a_ob) = abstract a in
-    let (b_mem, b_ob) = abstract b in
-    let res_mem = merge_rels lca_mem a_mem b_mem PairSet.diff PairSet.inter PairSet.union in
-    let res_ob_h = merge_rels lca_ob a_ob b_ob PairPairSet.diff PairPairSet.inter PairPairSet.union in
-    let res_ob = PairPairSet.inter res_ob_h (r_cross_sets res_mem res_mem) in
-    (res_mem, res_ob)
+let merge_r lca a b =
+  let (lca_mem, lca_ob) = abstract lca in
+  let (a_mem, a_ob) = abstract a in
+  let (b_mem, b_ob) = abstract b in
+  let res_mem = merge_rels lca_mem a_mem b_mem PairSet.diff PairSet.inter PairSet.union in
+  let res_ob_h = merge_rels lca_ob a_ob b_ob PairPairSet.diff PairPairSet.inter PairPairSet.union in
+  let res_ob = PairPairSet.inter res_ob_h (r_cross_sets res_mem res_mem) in
+  (res_mem, res_ob)
 
-  let sort_pair a b =  if a < b then (a, b) else (b, a)
+let sort_pair a b =  if a < b then (a, b) else (b, a)
 
-  exception CyclicGraph: (int * int) list -> exn
+exception CyclicGraph: (Z.t * Z.t) list -> exn
 
-  let dfs graph visited start =
-    let rec explore path visited node =
-      if List.mem node path then (Printf.printf "Cycle found!\n";
-                                  List.iter (fun x -> Printf.printf "(%d, %d) -> " (fst x) (snd x)) path;
-                                  raise (CyclicGraph path)) else
-      if List.mem node visited then visited else
-        let new_path = (path @ [node]) in
-        let edges = List.assoc node graph in
-        let visited = List.fold_left (fun visited node -> explore new_path visited node) visited edges in
-        (visited @ [node])
-    in explore [] visited start
+let dfs graph visited start =
+  let rec explore path visited node =
+    if List.mem node path then (Printf.printf "Cycle found!\n";
+                                List.iter (fun x -> Printf.printf "(%d, %d) -> " (Z.to_int (fst x)) (Z.to_int (snd x))) path;
+                                raise (CyclicGraph path)) else
+    if List.mem node visited then visited else
+      let new_path = (path @ [node]) in
+      let edges = List.assoc node graph in
+      let visited = List.fold_left (fun visited node -> explore new_path visited node) visited edges in
+      (visited @ [node])
+  in explore [] visited start
 
-  let topological_sort adj_list =
-    List.fold_left (fun visited (node, _) -> dfs adj_list visited node) [] adj_list
+let topological_sort adj_list =
+  List.fold_left (fun visited (node, _) -> dfs adj_list visited node) [] adj_list
 
-  let to_adj_list (vertices, edges) =
-    PairSet.fold
-      (fun x acc -> acc @ [(x, PairSet.elements (PairSet.filter (fun y -> x <> y && PairPairSet.mem (x, y) edges) vertices))]) vertices []
+let to_adj_list (vertices, edges) =
+  PairSet.fold
+    (fun x acc -> acc @ [(x, PairSet.elements (PairSet.filter (fun y -> x <> y && PairPairSet.mem (x, y) edges) vertices))]) vertices []
 
-  let concretize (r_mem, r_ob) =
-    if r_ob = PairPairSet.empty then (PairSet.elements r_mem, []) else
-      let ord_ob = PairSet.fold (fun x acc ->
-          PairSet.fold (fun y acc0 -> if (PairPairSet.mem (x, y) acc0 || PairPairSet.mem (y, x) acc0) then acc0
-                         else PairPairSet.add (sort_pair x y) acc0) (PairSet.filter (fun a -> a <> x) r_mem) acc) r_mem r_ob in
-      let adj_list = to_adj_list (r_mem, ord_ob) in
-      let front = topological_sort adj_list in
-      (List.rev front, [])
+let concretize (r_mem, r_ob) =
+  if r_ob = PairPairSet.empty then S (PairSet.elements r_mem, []) else
+    let ord_ob = PairSet.fold (fun x acc ->
+        PairSet.fold (fun y acc0 -> if (PairPairSet.mem (x, y) acc0 || PairPairSet.mem (y, x) acc0) then acc0
+                       else PairPairSet.add (sort_pair x y) acc0) (PairSet.filter (fun a -> a <> x) r_mem) acc) r_mem r_ob in
+    let adj_list = to_adj_list (r_mem, ord_ob) in
+    let front = topological_sort adj_list in
+    S (List.rev front, [])
 
-  let merge lca a b = concretize (merge_r lca a b)
-
-end
+let (merge: s -> s -> s -> s) = fun lca a b -> concretize (merge_r lca a b)
 
