experiments/orset/Quark_Orset.ml
@@ -1,55 +1,54 @@
-module Orset : sig
-  type t
-  type op = Add of int | Rem of int
-  val empty : t
-  val is_mem : int -> t -> bool
-  val app_op : (int * op) -> t -> t
-  val merge : t -> t -> t -> t
+module IntSet = Set.Make(Int)
+
+module Pair: sig
+  include Set.OrderedType
+  type t = (Z.t * Z.t)
+  val compare: t -> t -> int
 end = struct
-  module IntSet = Set.Make(Int)
-
-  module Pair: sig
-    include Set.OrderedType
-    val make: (int * int) -> t
-    val unmake: t -> (int * int)
-  end = struct
-    type t = (int * int)
-    let compare a b = if a = b then 0 else (if (fst a > fst b) || ((fst a = fst b) && (snd a > snd b)) then 1 else -1)
-    let make a = a
-    let unmake a = a
-  end
-
-  module PairSet = Set.Make(Pair)
-
-  type t = (int * int) list
-  type op = Add of int | Rem of int
-
-  let empty = []
-  let is_mem x s = List.exists (fun y -> snd y = x) s
-  let add x s = if is_mem (snd x) s then s else x::s
-  let rem x s = List.filter (fun y -> snd y <> x) s
-
-  let app_op op st = match op with
-    | (id, Add x) -> add (id, x) st
-    | (_, Rem x) -> rem x st
-
-  let abstract st = List.fold_left (fun acc x -> PairSet.add (Pair.make x) acc) PairSet.empty st
-
-  let concretize m_set = PairSet.fold (fun x acc -> (Pair.unmake x)::acc) m_set []
-
-  let merge_r lca a b =
-    let ixn = (PairSet.inter (PairSet.inter a b) lca) in
-    let diff_a = PairSet.diff a lca in
-    let diff_b = PairSet.diff b lca in
-    PairSet.union (PairSet.union diff_a diff_b) ixn
-
-  let merge lca a b =
-    let lca_abs = abstract lca in
-    let a_abs = abstract a in
-    let b_abs = abstract b in
-    let r_abs = merge_r lca_abs a_abs b_abs in
-    concretize r_abs
-
+  type t = (Z.t * Z.t)
+  let compare a b = if a = b then 0 else (if (fst a > fst b) || ((fst a = fst b) && (snd a > snd b)) then 1 else -1)
 end
+
+module PairSet = Set.Make(Pair)
+
+type t = (Z.t * Z.t) list
+type op = Add of Z.t | Rem of Z.t
+
+let empty = []
+let is_mem x s = List.exists (fun y -> snd y = x) s
+
+let rec update_id new_id old_ele st = match st with
+  | [] -> []
+  | x::xs -> if (snd x) = old_ele then (new_id, (snd x))::xs else update_id new_id old_ele xs
+
+let add x s = if is_mem (snd x) s then (update_id (fst x) (snd x) s) else x::s
+let rem x s = List.filter (fun y -> snd y <> x) s
+
+let app_op st op = match op with
+  | (id, Add x) -> add (id, x) st
+  | (_, Rem x) -> rem x st
+
+let abstract st = List.fold_left (fun acc x -> PairSet.add x acc) PairSet.empty st
+
+let concretize m_set = PairSet.fold (fun x acc -> x::acc) m_set []
+
+let get_id ele st = fst (PairSet.choose (PairSet.filter (fun x -> snd x = ele) st))
+
+let merge_r lca a b =
+  let ixn = (PairSet.inter (PairSet.inter a b) lca) in
+  let diff_a = PairSet.diff a lca in
+  let diff_b = PairSet.diff b lca in
+  let la1 = PairSet.filter (fun x -> not (PairSet.exists (fun y -> (snd y = snd x)) diff_b)) diff_a in
+  let lb1 = PairSet.filter (fun x -> not (PairSet.exists (fun y -> (snd y = snd x)) diff_a)) diff_b in
+  let la2 = PairSet.filter (fun x -> (PairSet.exists (fun y -> snd y = snd x) diff_b) && get_id (snd x) a > get_id (snd x) b) diff_a in
+  let lb2 = PairSet.filter (fun x -> (PairSet.exists (fun y -> snd y = snd x) diff_a) && get_id (snd x) a > get_id (snd x) a) diff_b in
+  PairSet.union (PairSet.union (PairSet.union (PairSet.union ixn la1) lb1) la2) lb2
+
+let (merge: t -> t -> t -> t) = fun lca a b ->
+  let lca_abs = abstract lca in
+  let a_abs = abstract a in
+  let b_abs = abstract b in
+  let r_abs = merge_r lca_abs a_abs b_abs in
+  concretize r_abs
 
 
